unit tests for QUIC C API

apps/quicMinusNet/quic.c
@@ -69,7 +69,7 @@ int main(int argc, char **argv)
   // client write buffer (cumulative)
   size_t clen = 0;
   size_t cmax = 8*1024; // too much; we use < 1KB
-  char *c_buffer = malloc(clen);
+  char *c_buffer = malloc(cmax);
   
   // buffer for secrets and tickets
   quic_secret *qs = malloc(sizeof(quic_secret));
@@ -104,7 +104,7 @@ int main(int argc, char **argv)
         
         printf("client call clen=%4d slen=%4d\n", clen, slen);
         rc = FFI_mitls_quic_process(client, s_buffer, &slen, c_buffer, &clen, &errmsg);
-        printf("client done clen=%4d slen=%4d r=%s\n", clen, slen, quic_result_string(rc));
+        printf("client done clen=%4d slen=%4d status=%s\n", clen, slen, quic_result_string(rc));
         dump(c_buffer, clen);
         
         client_complete |= rc == TLS_client_complete || rc == TLS_client_complete_with_early_data;
@@ -125,7 +125,7 @@ int main(int argc, char **argv)
 
         printf("server call clen=%4d slen=%4d\n", clen, slen);
         rs = FFI_mitls_quic_process(server, c_buffer, &clen, s_buffer, &slen, &errmsg);
-        printf("sender done clen=%4d slen=%4d r=%s\n", clen, slen, quic_result_string(rs));
+        printf("sender done clen=%4d slen=%4d status=%s\n", clen, slen, quic_result_string(rs));
         dump(s_buffer, slen);
 
         server_complete |= rs == TLS_server_complete;
@@ -169,14 +169,14 @@ int main(int argc, char **argv)
     c_buffer += clen; cmax -= clen; clen = cmax;
     rc = FFI_mitls_quic_process(client, s_buffer, &slen, c_buffer, &clen, &errmsg);
     assert(rc == TLS_would_block);
-    printf("client done clen=%4d slen=%4d r=%s\n", clen, slen, quic_result_string(rc));
+    printf("client done clen=%4d slen=%4d status=%s\n", clen, slen, quic_result_string(rc));
     printf("ClientHello[%4d] ---->\n\n",clen);
       
     s_buffer += slen; smax -= slen; slen = smax;
     rs = FFI_mitls_quic_process(server, c_buffer, &clen, s_buffer, &slen, &errmsg);
     assert(rs == TLS_server_accept);
     FFI_mitls_quic_get_exporter(server, 0, qs, &errmsg);
-    printf("server done clen=%4d slen=%4d r=%s\n", clen, slen, quic_result_string(rs));
+    printf("server done clen=%4d slen=%4d status=%s\n", clen, slen, quic_result_string(rs));
     printf("server secret is "); dump(qs->secret, 32);
     printf("                  <---- ServerHello;(EE; Cert; CertVerify; Finished)[%4d]\n\n",slen);
 
@@ -184,27 +184,27 @@ int main(int argc, char **argv)
     rc = FFI_mitls_quic_process(client, s_buffer, &slen, c_buffer, &clen, &errmsg);
     assert(rc == TLS_client_complete);
     FFI_mitls_quic_get_exporter(client, 0, qs, &errmsg);
-    printf("client done clen=%4d slen=%4d r=%s\n", clen, slen, quic_result_string(rc));
+    printf("client done clen=%4d slen=%4d status=%s\n", clen, slen, quic_result_string(rc));
     printf("client secret is "); dump(qs->secret, 32);
     printf("(Finished) [%4d] ---->\n\n",clen);
       
     s_buffer += slen; smax -= slen; slen = smax;
     rs = FFI_mitls_quic_process(server, c_buffer, &clen, s_buffer, &slen, &errmsg);
     assert(rs == TLS_server_complete);
-    printf("server done clen=%4d slen=%4d r=%s\n", clen, slen, quic_result_string(rs));
+    printf("server done clen=%4d slen=%4d status=%s\n", clen, slen, quic_result_string(rs));
 
-    // NB calling the server again to get the ticket
+    // NB we must call the server again to get a ticket
     c_buffer += clen; cmax -= clen; clen = 0;
     s_buffer += slen; smax -= slen; slen = smax;
     rs = FFI_mitls_quic_process(server, c_buffer, &clen, s_buffer, &slen, &errmsg);
     assert(rs == TLS_would_block);
-    printf("server done clen=%4d slen=%4d r=%s\n", clen, slen, quic_result_string(rs));
+    printf("server done clen=%4d slen=%4d status=%s\n", clen, slen, quic_result_string(rs));
     printf("                  <---- {Ticket}[%4d]\n\n", slen);
 
     clen = cmax;
     rc = FFI_mitls_quic_process(client, s_buffer, &slen, c_buffer, &clen, &errmsg);
     assert(rc == TLS_would_block);
-    printf("client done clen=%4d slen=%4d r=%s\n", clen, slen, quic_result_string(rc));
+    printf("client done clen=%4d slen=%4d status=%s\n", clen, slen, quic_result_string(rc));
 
     if(FFI_mitls_quic_get_ticket(client, qt, &errmsg))
     {
@@ -212,6 +212,35 @@ int main(int argc, char **argv)
       dump(qt->ticket, qt->len);
     }
     else printf("Failed to get ticket: %s\n", errmsg);
+
+    printf("\n     TICKET-BASED RESUMPTION\n\n");
+    
+    FFI_mitls_quic_free(server);
+    FFI_mitls_quic_free(client);
+    
+    printf("server create\n");
+    if(!FFI_mitls_quic_create(&server, &config, &errmsg))
+      {
+        printf("quic_create server failed: %s\n", errmsg);
+        return -1;
+      }
+    config.is_server = 0;
+    config.host_name = "localhost";
+    config.ticket = *qt;
+    
+    printf("client create\n");
+    if(!FFI_mitls_quic_create(&client, &config, &errmsg))
+      {
+        printf("quic_create client failed: %s\n", errmsg);
+        return -1;
+      }
+
+    s_buffer += slen; smax -= slen; slen = 0;
+    c_buffer += clen; cmax -= clen; clen = cmax;
+    rc = FFI_mitls_quic_process(client, s_buffer, &slen, c_buffer, &clen, &errmsg);
+    printf("client done clen=%4d slen=%4d status=%s\n", clen, slen, quic_result_string(rc));
+    assert(rc == TLS_client_early);
+    printf("ClientHello[%4d] ---->\n\n",clen);
   }
 
   FFI_mitls_quic_free(server);
